src/Generated/AwsEncryptionSdk.dfy
@@ -15,28 +15,43 @@ module {:extern "Dafny.Aws.Esdk"} Aws.Esdk {
         nameonly keyring: Crypto.IKeyring?,
         nameonly materialsManager: Crypto.ICryptographicMaterialsManager?
     )
+    {
+        predicate Valid() {
+            true 
+        }
+    }
 
     datatype EncryptOutput = EncryptOutput(
         nameonly ciphertext: seq<uint8>,
         nameonly encryptionContext: Crypto.EncryptionContext,
         nameonly algorithmSuite: Crypto.AlgorithmSuite
     )
+    {
+        predicate Valid() {
+            true 
+        }
+    }
 
     datatype DecryptInput = DecryptInput(
         nameonly ciphertext: seq<uint8>,
         nameonly keyring: Crypto.IKeyring?,
         nameonly materialsManager: Crypto.ICryptographicMaterialsManager?
     )
+    {
+        predicate Valid() {
+            true 
+        }
+    }
 
     datatype DecryptOutput = DecryptOutput(
         nameonly plaintext: seq<uint8>,
         nameonly encryptionContext: Crypto.EncryptionContext,
         nameonly algorithmSuite: Crypto.AlgorithmSuite
     )
-
-    trait IAwsEncryptionSdkClient {
-        method Encrypt(input: EncryptInput) returns (res: Result<EncryptOutput, string>)
-        method Decrypt(input: DecryptInput) returns (res: Result<DecryptOutput, string>)
+    {
+        predicate Valid() {
+            true 
+        }
     }
 
     datatype AwsEncryptionSdkClientConfig = AwsEncryptionSdkClientConfig(
@@ -44,24 +59,17 @@ module {:extern "Dafny.Aws.Esdk"} Aws.Esdk {
         nameonly maxEncryptedEdks: int,
         nameonly configDefaults: string
     )
-
-    class AwsEncryptionSdkClient extends IAwsEncryptionSdkClient {
-        const clientConfig: AwsEncryptionSdkClientConfig
-
-        constructor(clientConfig: AwsEncryptionSdkClientConfig) {
-            this.clientConfig := clientConfig;
+    {
+        predicate Valid() {
+            true
         }
+    }
 
-        static method createClient(nameonly clientConfig: AwsEncryptionSdkClientConfig) returns (res: AwsEncryptionSdkClient) {
-            res := new AwsEncryptionSdkClient(clientConfig);
-        }
-
-        method Encrypt(input: EncryptInput) returns (res: Result<EncryptOutput, string>) {
-            // TODO
-        }
-
-        method Decrypt(input: DecryptInput) returns (res: Result<DecryptOutput, string>) {
-            // TODO
-        }
+    trait IAwsEncryptionSdkClient {
+        method Encrypt(input: EncryptInput) returns (res: Result<EncryptOutput, string>)
+            requires input.Valid()
+        method Decrypt(input: DecryptInput) returns (res: Result<DecryptOutput, string>)
+            requires input.Valid()
+        static method {:extern "createClient"} createClient(clientConfig: AwsEncryptionSdkClientConfig) returns (res: IAwsEncryptionSdkClient)
     }
 }
